Automata/Collapse.lean
@@ -32,14 +32,14 @@ theorem collapse_eval (dfa : DFA (Fin (n + 1) → α) state) (i : Fin (n + 1)) (
   : dfa.eval (l.map (recover_index i k)) = (collapse i k dfa).eval l := collapse_evalFrom dfa i k l dfa.start
 
 theorem collapse_correct (dfa : DFA (Fin (n + 1) → Fin (b + 2)) state) (l : Fin (n+1) → ℕ) (i : Fin (n + 1)) (k: Fin n)  (hl : l i = l k) (hik : i.val > k.val) :
-  dfa.eval (toWord l b) = (collapse i k dfa).eval ((toWord l b).map (remove_index i)) := by
+  dfa.eval (toWord l b) = (collapse i k dfa).eval ((toWord l b).map (Fin.removeNth i)) := by
   rw[← collapse_eval]
   congr
 
   have := @eqInput_if_equal (n+1) (b) l i k
 
   simp only [List.map_map]
-  suffices : ∀ v ∈ toWord l b, (recover_index i k ∘ remove_index i) v = v
+  suffices : ∀ v ∈ toWord l b, (recover_index i k ∘ Fin.removeNth i) v = v
   .
     ext j v
     constructor
@@ -56,15 +56,16 @@ theorem collapse_correct (dfa : DFA (Fin (n + 1) → Fin (b + 2)) state) (l : Fi
   intro v hv
   dsimp only [Function.comp_apply]
   -- rw[recover_remove]
-  rw[recover_index, insert_remove]
-  rw[remove_index, Fin.removeNth, Fin.succAbove, Fin.castSucc, Fin.castAdd, Fin.castLE]
+  simp[recover_index, Fin.removeNth, Fin.succAbove, Fin.castSucc, Fin.castAdd, Fin.castLE]
   specialize this hl v
   split;
   . simp_all only [Fin.getElem_fin, gt_iff_lt, Fin.eta]
     ext : 1
+    simp_all [Fin.insert, Function.update]
+    intro a
+    subst a
+    ext : 1
     simp_all only
-    congr
-    simp_all only [Fin.coe_eq_castSucc, forall_const]
     rfl
   . rename_i h
     have : ¬ k.val < i := by
@@ -80,7 +81,7 @@ theorem collapse_respectZero (dfa : DFA (Fin (n + 1) → Fin (b + 2)) state) (i 
 
 -- Auxilliary functions for collapse
 
--- def remove_index (i : Fin (n + 1)) (f: Fin (n + 1) → α):
+-- def @Fin.removeNth (i : Fin (n + 1)) (f: Fin (n + 1) → α):
 --    (Fin n → α) :=
 --     fun j => f (if j.val < i.val then j else ⟨j.val + 1, by omega⟩)
 
@@ -89,9 +90,9 @@ theorem collapse_respectZero (dfa : DFA (Fin (n + 1) → Fin (b + 2)) state) (i 
 --     fun j => if hlt : j < i then f ⟨j, by omega⟩ else if hgt : j > i then f ⟨j - 1, by omega⟩ else f k
 
 -- theorem remove_recover (i : Fin (n + 1)) (k: Fin n) (f: Fin n → α) :
---   remove_index i (recover_index i k f) = f := by
+--   @Fin.removeNth i (recover_index i k f) = f := by
 --   ext x
---   simp[remove_index, recover_index]
+--   simp[@Fin.removeNth, recover_index]
 --   split; simp only [Fin.coe_castSucc, Fin.eta, dite_eq_ite, ite_eq_then, not_lt]
 --   . intro h
 --     have : i.val ≤ x.val := by exact h
@@ -114,9 +115,9 @@ theorem collapse_respectZero (dfa : DFA (Fin (n + 1) → Fin (b + 2)) state) (i 
 --         omega
 
 -- theorem recover_remove (i : Fin (n + 1)) (k: Fin n) (f: Fin (n + 1) → α) (hf: f i = f k) (hik : i.val > k.val ) :
---   recover_index i k (remove_index i f) = f := by
+--   recover_index i k (@Fin.removeNth i f) = f := by
 --   ext x
---   simp[remove_index, recover_index]
+--   simp[@Fin.removeNth, recover_index]
 --   split; simp only [Fin.coe_castSucc, Fin.eta, dite_eq_ite, ite_eq_then, not_lt]
 --   . split; simp_all
 --     . split
