Automata/Demos.lean
@@ -10,37 +10,53 @@ theorem zero_is_zero : 0 = 0 := by
   apply (eqBase_iff_equal 0 2 (fun _ => 0) 0 1).mpr
   native_decide
 
+#eval (project 1 (eqBase 0 2 0 1)).fixLeadingZeros.eval (toWord ![1] 0)
 
 theorem foo : 100000 = 100000 := by
   apply (eqBase_iff_equal 0 2 (fun _ => 100000) 0 1).mpr
   native_decide
 
 theorem pro : ∃ (x : ℕ), x = 0 := by
-  have : ∀ x : ℕ, x = 0 ↔ (eqBase 0 2 0 1).eval (toWord (recover_value 0 x (fun _ => 0)) 0) := by
+
+  have : ∀ x : ℕ, x = 0 ↔ (eqBase 0 2 0 1).eval (toWord (Fin.insertNth 0 x (fun _ => 0)) 0) := by
     intro x
-    have := eqBase_iff_equal 0 2 (recover_value 0 x (fun _ => 0)) 0 1
-    simp[recover_value, Fin.insert] at this
-    simp[recover_value, Fin.insert]
+    have := eqBase_iff_equal 0 2 (Fin.insertNth 0 x (fun _ => 0)) 0 1
+    simp[Fin.insertNth, Fin.insert] at this
+    simp[Fin.insertNth, Fin.insert]
     exact this
 
-  -- rw[this]
+  simp only [this]
 
-  have : ∃ (x : ℕ), DFAO.eval (eqBase 0 2 0 1) (toWord (recover_value 0 x (fun _ => 0)) 0) = true := by
+  have : ∃ (x : ℕ), DFAO.eval (eqBase 0 2 0 1) (toWord (Fin.insertNth 0 x (fun _ => 0)) 0) = true := by
     refine (project_iff (fun x ↦ 0) 0 (eqBase 0 2 0 1) ?_).mp ?_
     . exact equality_respectZero
     . native_decide
 
   rcases this with ⟨x, hx⟩
   use x
-  rw[this]
-  exact hx
 
-theorem prox : ∃ (x : ℕ), x = x := by
-  have : ∀ x : ℕ, x = x ↔ (eqBase 0 2 0 1).eval (toWord (recover_value 1 x (recover_value 0 x (fun _ => 1))) 0) := by
+theorem proxy : ∃ x : ℕ, ∃ y, x = y := by
+  have : ∀ x y : ℕ, x = y ↔ (eqBase 0 2 0 1).eval (toWord ![x, y] 0 ) := by
+    intro x y
+    have := eqBase_iff_equal 0 2 ![x, y] 0 1
+    exact this
+  simp_rw [this]
+  have : ∀ x, ((∃ y, (eqBase 0 2 0 1).eval (toWord ![x, y] 0)) ↔ (project 1 (eqBase 0 2 0 1)).fixLeadingZeros.eval (toWord ![x] 0)) := by
     intro x
-    have := eqBase_iff_equal 0 2 (recover_value 1 x (recover_value 0 x (fun _ => 1))) 0 1
-    convert this
-  have : ∀ x : ℕ, (eqBase 0 2 0 1).eval (toWord (recover_value 1 x (recover_value 0 x (fun _ => 1))) 0) ↔ (collapse 1 0 (eqBase 0 2 0 1)).eval ((toWord (recover_value 1 x (recover_value 0 x (fun _ => 1))) 0).map (remove_index 1)) := by
-    intro x
+    have := project_iff ![x] 1 (eqBase 0 2 0 1) ?_
     sorry
   sorry
+
+
+#check exists_congr
+-- theorem prox : ∃ (x : ℕ), x = x := by
+--   have : ∀ x : ℕ, x = x ↔ (eqBase 0 2 0 1).eval (toWord (Fin.insertNth 1 x (Fin.insertNth 0 x (fun _ => 1))) 0) := by
+--     intro x
+--     have := eqBase_iff_equal 0 2 (Fin.insertNth 1 x (Fin.insertNth 0 x (fun _ => 1))) 0 1
+--     convert this
+
+--   apply exists_congr this |>.mpr
+--   have : ∀ x : ℕ, (eqBase 0 2 0 1).eval (toWord (Fin.insertNth 1 x (Fin.insertNth 0 x (fun _ => 1))) 0) ↔ (collapse 1 0 (eqBase 0 2 0 1)).eval ((toWord (Fin.insertNth 1 x (Fin.insertNth 0 x (fun _ => 1))) 0).map (remove_index 1)) := by
+--     intro x
+--     sorry
+--   sorry
