Automata/Equality_new.lean
@@ -1,0 +1,379 @@
+import Mathlib.Tactic
+import Mathlib.Data.List.Basic
+import Automata.DFA
+import Automata.NFA
+import Automata.Input_new
+import Automata.Boolean
+import Automata.Replicate
+import Automata.LeadingZeros
+import Mathlib.Data.Nat.Digits
+
+-- The equality checking automata for two numbers in a long list of inputs.
+def eqBase (k n: ℕ) (a b : Fin n): DFA (Fin n → Fin (k+2)) (Fin 2) := {
+  transition := fun f s => match s with
+    | 0 => if (f a).val == f b then 0 else 1
+    | 1 => 1
+  start := 0
+  output := fun x => x == 0
+}
+
+/- Try to prove eqBase is correct
+
+1. DFA accepts iff f 0 = f 1 for all f ∈ input
+2. input natural numbers are equal iff f 0 = f 1 for all f ∈ input
+
+-/
+
+--Start of Step 1
+--Right to Left
+theorem eqBase_if_equal_aux (input: List (Fin n → Fin (k+2))):
+  (∀ f ∈ input, (f a).val = f b) → (eqBase k n a b).evalFrom input 0 := by
+  intro h
+  induction input
+  case nil =>
+    simp[eqBase, DFAO.evalFrom, DFAO.transFrom]
+  case cons f fs ih =>
+    have h1 := h f
+    simp only [List.mem_cons, true_or, Fin.isValue, true_implies] at h1
+    simp only [DFAO.evalFrom, DFAO.transFrom, Fin.isValue]
+    have: ((eqBase k n a b).transition f 0) = 0 := by
+      simp only [eqBase, Fin.isValue, beq_iff_eq, h1, ↓reduceIte]
+    rw[this]
+    apply ih
+    intro f' hf'
+    apply h
+    simp only [List.mem_cons, or_true, hf']
+
+
+-- Left to right, much harder
+theorem eqBase_trans_zero (state : Fin 2) (f : Fin n → Fin (k+2)) :
+  (eqBase k n a b).transition f state = 0 ↔ state = 0 ∧ (f a).val = f b := by
+  simp only [eqBase, Fin.isValue, beq_iff_eq]
+  split <;> simp
+
+
+theorem eqBase_transFrom_zero (state: Fin 2) (l : List (Fin n → Fin (k+2))) :
+  (eqBase k n a b).transFrom l state = 0 ↔ state = 0 ∧ ∀ f ∈ l, (f a).val = f b := by
+  induction l generalizing state
+  case nil =>
+    simp[eqBase, DFAO.transFrom]
+  case cons f fs ih =>
+    simp[DFAO.transFrom]
+    specialize ih ((eqBase k n a b).transition f state)
+    constructor
+    . intro h
+      have:= ih.mp h
+      rcases this with ⟨h1, h2⟩
+      have:= (eqBase_trans_zero state f).mp h1
+      rcases this with ⟨h3, h4⟩
+      exact ⟨h3, ⟨h4, h2⟩⟩
+    . intro h
+      rcases h with ⟨h1, h2, h3⟩
+      apply ih.mpr
+      constructor
+      . apply (eqBase_trans_zero state f).mpr
+        exact ⟨h1, h2⟩
+      . exact h3
+
+theorem eqInput_if_eqBase_aux (input: List (Fin n → Fin (k+2))):
+  (eqBase k n a b).transFrom input 0 = 0 → (∀ f ∈ input, (f a).val = f b) := by
+  intro h
+  exact (eqBase_transFrom_zero 0 input).mp h |>.2
+
+theorem eqInput_if_eqBase (input: List (Fin n → Fin (k+2))):
+  (eqBase k n a b).evalFrom input 0 → (∀ f ∈ input, (f a).val = f b) := by
+  intro h
+  have:= eqInput_if_eqBase_aux (b := b) (a := a) input
+  apply this
+  -- simp[DFAO.evalFrom, eqBase] at h
+  simp_all only [DFAO.evalFrom, eqBase, beq_iff_eq, true_implies]
+
+-- End of Left to right, final step 1 statement:
+theorem eqBase_iff_eqInput (k : ℕ) (input: List (Fin n → Fin (k+2))):
+  (eqBase k n a b).eval input ↔ (∀ f ∈ input, (f a).val = f b) := by
+  constructor
+  . apply eqInput_if_eqBase input
+  . apply eqBase_if_equal_aux input
+
+
+--An Auxillary theorem for left to right
+theorem eqZipOfIndexEq (lsLength : ℕ) (lss: Fin l → (List ℕ))
+      (hlb: ∀ x : Fin l, ∀ ls ∈ lss x, ls < k+2 ) (m n : Fin l)
+      (hls: ∀ x : Fin l, (lss x).length = lsLength) (hIndexEq: ∀i, ∀ (hi : i < lsLength), (lss m)[i]'(by
+        specialize hls m
+        exact Nat.lt_of_lt_of_eq hi (id (Eq.symm hls))
+      ) = (lss n)[i]'(by
+        specialize hls n
+        exact Nat.lt_of_lt_of_eq hi (id (Eq.symm hls))
+      )): ∀ f ∈ (@zip l k lsLength lss hlb hls), (f m).val = f n:= by
+      intro f hf
+      induction lsLength generalizing lss
+      case zero =>
+        simp only [zip, List.not_mem_nil] at hf
+      case succ lsLength ih =>
+        simp only [zip, Fin.getElem_fin, List.mem_cons] at hf
+        rcases hf with hf | hf
+        . specialize hIndexEq 0 (by norm_num)
+          simp[hf, hIndexEq]
+        . apply ih (fun i ↦ (lss i).tail)
+          . intro i hi
+            rw[List.getElem_tail, List.getElem_tail]
+            apply hIndexEq
+            simp only [add_lt_add_iff_right]
+            exact hi
+          . exact hf
+
+theorem eqInput_if_equal (input : Fin l → ℕ) (m n : Fin l) :
+  input m = input n →  ∀ f ∈ toWord input k, (f m).val = (f n) := by
+    intro h
+
+    have stretchLenEq: (stretchLen (mapToBase (k+2) input)) m =
+    (stretchLen (mapToBase (k+2) input)) n := by
+      simp_all[stretchLen, mapToBase, h]
+
+    have lenStretchLen0 : ((stretchLen (mapToBase (k+2) input)) m).length = maxLenFin (mapToBase (k+2) input) := by
+      apply stretchLen_uniform
+
+    have lenStretchLen1 : ((stretchLen (mapToBase (k+2) input)) n).length = maxLenFin (mapToBase (k+2) input) := by
+      apply stretchLen_uniform
+
+    have stretchLenIndexEq (i: ℕ)(hi: i < (maxLenFin (mapToBase (k+2) input))): (stretchLen (mapToBase (k+2) input) m)[i] = (stretchLen (mapToBase (k+2) input) n)[i] := by
+      simp only [stretchLenEq]
+
+    intro f hf
+    rw[toWord] at hf
+    apply eqZipOfIndexEq (maxLenFin (mapToBase (k+2) input)) (stretchLen (mapToBase (k+2) input))
+    . apply stretchLenIndexEq
+    . exact hf
+
+--Right to left
+theorem equal_if_toBaseEq: toBase b m = toBase b n → m = n := by
+  intro h
+  rw[← ofBase_toBase b n, ← ofBase_toBase b m]
+  congr
+
+theorem equal_if_mapToBaseEq (input: Fin l → ℕ) (m n : Fin l) :
+  (mapToBase (k+2) input m) = (mapToBase (k+2) input n) → input m = input n := by
+  intro h
+  simp only [mapToBase] at h
+  apply equal_if_toBaseEq
+  exact h
+
+theorem eq_if_addZeroesEq_nonzero (n: ℕ) (L: Fin l → (List ℕ)) (k p: Fin l) (hn: n ≥ maxLenFin L)  (lenk :0 < (L k).length) (hk: (L k)[0] ≠ 0) (lenp :0 < (L p).length) (hp: (L p)[0] ≠ 0) :
+  addZeroes (n - (L k).length) (L k) = addZeroes (n - (L p).length) (L p) → (L k) = (L p):= by
+  intro h
+  simp only [maxLen, zero_le, max_eq_left, ge_iff_le, max_le_iff] at hn
+  have kLen: (L k).length ≤ n := by
+    trans maxLenFin L
+    apply len_le_maxLen
+    refine (List.mem_ofFn L (L k)).mpr ?_
+    exact exists_apply_eq_apply L k
+    exact hn
+  have pLen : (L p).length ≤ n := by
+    trans maxLenFin L
+    apply len_le_maxLen
+    refine (List.mem_ofFn L (L p)).mpr ?_
+    exact exists_apply_eq_apply L p
+    exact hn
+
+  have hL: n - (L k).length = n - (L p).length := by
+    by_contra hL
+    have hLen: n - (L k).length < n - (L p).length ∨ n - (L k).length > n - (L p).length := by
+      exact Nat.lt_or_gt_of_ne hL
+    have kAddLen: (addZeroes (n - (L k).length) (L k)).length = n := by simp only [addZeroesLength]; omega
+    have lAddLen: (addZeroes (n - (L p).length) (L p)).length = n :=  by simp only [addZeroesLength]; omega
+    rcases hLen with (hLen | hLen)
+    .
+      have addl : (addZeroes (n - (L p).length) (L p))[n-(L k).length] = 0 := by
+        simp[addZeroes]
+        apply List.getElem_of_replicate_append_left
+        exact hLen
+
+      have addk : (addZeroes (n - (L k).length) (L k))[n - (L k).length] ≠  0 := by
+        simp[addZeroes]
+        rw[List.getElem_append_right]
+        simp only [List.length_replicate, le_refl, tsub_eq_zero_of_le]
+        exact hk
+        . simp[*]
+      simp_all only [ne_eq, ge_iff_le, not_true_eq_false]
+    .
+      have addk : (addZeroes (n - (L k).length) (L k))[n-(L p).length] = 0 := by
+        simp[addZeroes]
+        apply List.getElem_of_replicate_append_left
+        exact hLen
+      have addl : (addZeroes (n - (L p).length) (L p))[n-(L p).length] ≠  0 := by
+        simp only [addZeroes, ne_eq]
+        rw[List.getElem_append_right]
+        simp only [List.length_replicate, le_refl, tsub_eq_zero_of_le]
+        exact hp
+        . simp
+      simp_all only [ge_iff_le, ne_eq]
+  rw[← hL] at h
+  simp only [addZeroes, List.append_cancel_left_eq] at h
+  exact h
+
+theorem contra (input : Fin l → ℕ) (m n : Fin l) (h : (stretchLen (mapToBase (k+2) input) m) = (stretchLen (mapToBase (k+2) input) n)) (hn: input n = 0) (hm : input m ≠ 0) : False := by
+  simp[stretchLen, mapToBase, toBase, hn] at h
+  have : ∀ x ∈ addZeroes (maxLenFin (mapToBase (k+2) input)) [], x = 0 ∨ x ∈ [] := by
+    apply addZeroes_elem
+  simp only [List.not_mem_nil, or_false] at this
+  rw[← h] at this
+  have hbm: ∀x ∈ (toBase (k+2) (input m)), x = 0 := by
+    intro x hx
+    apply this
+    simp only [addZeroes, le_add_iff_nonneg_left, zero_le, List.mem_append, List.mem_replicate,
+      ne_eq, List.mem_reverse]
+    right
+    exact List.mem_reverse.mp hx
+  have: input m > 0 := by exact Nat.zero_lt_of_ne_zero hm
+  have hPos := toBase_lead_nonzero (k+2) (input m) (by omega) this
+  specialize hbm ((toBase (k+2) (input m))[0]'(by
+      apply toBase_len_nonzero <;> omega
+  ))
+  have hyp : (toBase (k+2) (input m))[0]'(by
+  have:= toBase_len_nonzero (k+2) (input m) (by omega) (by omega)
+  omega) ∈ toBase (k+2) (input m) := by apply List.getElem_mem
+  specialize hbm hyp
+  rw[hbm] at hPos
+  contradiction
+
+theorem eq_if_stretchLenEq (input : Fin l → ℕ)  (m n : Fin l) :
+  (stretchLen (mapToBase (k+2) input) m) = (stretchLen (mapToBase (k+2) input) n) → input m = input n := by
+  intro h
+  apply equal_if_mapToBaseEq
+  by_cases hm: input m = 0
+  . by_cases hn : input n = 0
+    . simp[mapToBase, hn, hm]
+    . by_contra; apply contra; exact h.symm; exact hm; exact hn
+  by_cases hn: input n = 0
+  . by_contra; apply contra; exact h; exact hn; exact hm
+  apply eq_if_addZeroesEq_nonzero (maxLenFin (mapToBase (k+2) input)) (mapToBase (k+2) input) m n
+  . simp only [ge_iff_le]; rfl
+  . simp only [mapToBase, List.map_cons, List.map_nil, List.getElem_cons_zero, ne_eq]
+    refine Nat.ne_zero_iff_zero_lt.mpr ?_
+    apply toBase_lead_nonzero
+    simp_all only [Fin.getElem_fin, ge_iff_le, le_add_iff_nonneg_left, zero_le]
+    . omega
+  . simp only [mapToBase, List.map_cons, List.map_nil, List.getElem_cons_zero, ne_eq]
+    refine Nat.ne_zero_iff_zero_lt.mpr ?_
+    apply toBase_lead_nonzero
+    simp_all only [Fin.getElem_fin, ge_iff_le, le_add_iff_nonneg_left, zero_le]
+    . omega
+  . simp_all[stretchLen]
+  . simp only [mapToBase, Fin.getElem_fin, List.getElem_map]
+    apply toBase_len_nonzero <;> omega
+  . simp only [mapToBase, Fin.getElem_fin, List.getElem_map]
+    apply toBase_len_nonzero <;> omega
+
+theorem indexEqOfEqZip (lsLength : ℕ) (lss: Fin l → (List ℕ))
+      (hlb: ∀ x : Fin l, ∀ ls ∈ lss x, ls < k+2 ) (m n : Fin l)
+      (hls: ∀ x : Fin l, (lss x).length = lsLength) :
+      (∀f ∈ (@zip l k lsLength lss hlb hls), (f m).val = f n)
+      → ∀i, ∀ (hi : i < lsLength), (lss m)[i]'(by
+        specialize hls m
+        exact Nat.lt_of_lt_of_eq hi (id (Eq.symm hls))
+      ) = (lss n)[i]'(by
+        specialize hls n
+        exact Nat.lt_of_lt_of_eq hi (id (Eq.symm hls))
+      ) := by
+        intro h
+        induction lsLength generalizing lss
+        case zero => intro i hi; contradiction
+        case succ s ih =>
+          intro i hi
+          simp [zip, Fin.getElem_fin, List.mem_cons, Fin.isValue,
+            forall_eq_or_imp, Fin.val_zero, Fin.val_one] at h
+          rcases h with ⟨h1, h2⟩
+          specialize ih (fun i ↦ (lss i).tail)
+          specialize ih (zipTailHlb lss hlb)
+          specialize ih (zipTailHls lss hls)
+          specialize ih h2
+          simp only [List.getElem_tail] at ih
+          match i with
+          | 0 => exact h1
+          | n + 1 =>
+            simp only [add_lt_add_iff_right] at hi
+            specialize ih n hi
+            exact ih
+
+theorem equal_if_eqInput (input : Fin l → ℕ) (m n : Fin l) :
+  (∀ f ∈ toWord input k, (f m).val = (f n)) → input m = input n := by
+    intro h
+    simp only [List.length_cons, List.length_singleton, Nat.reduceAdd, toWord, Fin.zero_eta,
+      Fin.isValue, Fin.mk_one] at h
+    apply @eq_if_stretchLenEq l k input m n
+    .
+      have inter := indexEqOfEqZip (maxLenFin (mapToBase (k+2) input))  (stretchLen (mapToBase (k+2) input)) (stretchLen_of_mapToBase_lt_base (k+2) input (by omega)) m n (by exact fun x ↦ stretchLen_uniform (mapToBase (k + 2) input) x)
+      specialize inter h
+      have:= stretchLen_uniform (mapToBase (k+2) input)
+      have len0 : ((stretchLen (mapToBase (k+2) input) m)).length = maxLenFin (mapToBase (k+2) input) := by
+        exact this m
+      have len1 : ((stretchLen (mapToBase (k+2) input) n)).length = maxLenFin (mapToBase (k+2) input) := by
+        exact this n
+      apply List.ext_getElem
+      . simp_all only
+      . intro _ _ _
+        apply inter
+        simp_all only [Fin.getElem_fin]
+
+-- Step 2 Complete
+theorem eqInput_iff_equal (input : Fin l → ℕ) (m n : Fin l) :
+  (∀ f ∈ toWord input k, (f m).val = (f n)) ↔ input m = input n := by
+    constructor
+    . apply equal_if_eqInput
+    . apply eqInput_if_equal
+
+-- Final theorem
+theorem eqBase_iff_equal (b l: ℕ) (input : Fin l → ℕ) (m n : Fin l):
+  input m = input n ↔ (eqBase b l m n).eval (toWord input b) := by
+  constructor
+  . intro h
+    refine (eqBase_iff_eqInput b (toWord input b)).mpr ?_
+    exact fun f a ↦ eqInput_if_equal input m n h f a
+  . intro h
+    rw[← eqInput_iff_equal]
+    exact fun f a ↦ eqInput_if_eqBase (toWord input b) h f a
+
+
+theorem equality_respectZero : (eqBase b l m n).respectZero := by
+  rw[DFA.respectZero]
+  intro x c
+  constructor
+  intro h
+  rw[padZeros]
+  rw[DFAO.eval, DFAO.evalFrom, DFAO.transFrom_of_append]
+  nth_rw 1 [eqBase]
+  simp only [Fin.isValue, beq_iff_eq]
+  suffices: (DFAO.transFrom (eqBase b l m n) (List.replicate c fun _ ↦ 0) (eqBase b l m n).start) = 0
+  . rw[this]
+    simp[DFAO.eval, DFAO.evalFrom] at h
+    nth_rw 1 3 [eqBase] at h
+    simp only [Fin.isValue, beq_iff_eq] at h
+    exact h
+  nth_rw 2 [eqBase]
+  simp only [Fin.isValue]
+  apply eqBase_transFrom_zero 0 (List.replicate c fun _ ↦ 0) |>.mpr
+  constructor
+  . rfl
+  . intro f a
+    simp_all only [List.mem_replicate, ne_eq, Fin.val_zero]
+  . intro h
+    contrapose h; simp_all only [Bool.not_eq_true]
+    rw[padZeros]
+    rw[DFAO.eval, DFAO.evalFrom, DFAO.transFrom_of_append]
+    nth_rw 1 [eqBase]
+    simp only [Fin.isValue, beq_iff_eq]
+    suffices: (DFAO.transFrom (eqBase b l m n) (List.replicate c fun _ ↦ 0) (eqBase b l m n).start) = 0
+    . rw[this]
+      simp[DFAO.eval, DFAO.evalFrom] at h
+      nth_rw 1 3 [eqBase] at h
+      simp only [Fin.isValue, beq_iff_eq] at h
+      exact h
+    nth_rw 2 [eqBase]
+    simp only [Fin.isValue]
+    apply eqBase_transFrom_zero 0 (List.replicate c fun _ ↦ 0) |>.mpr
+    simp_all only [Fin.isValue, List.mem_replicate, ne_eq, Fin.val_zero, and_imp, implies_true, and_self]
+
+
+
+-- Demos
